theories/rules/mov.v
@@ -64,7 +64,8 @@ Proof.
     rewrite (preserve_get_retri_gmap _ σ1).
     rewrite (preserve_inv_trans_hpool_consistent _ σ1).
     rewrite (preserve_inv_trans_pgt_consistent _ σ1).
-    rewrite (preserve_inv_trans_pg_num_ub _ σ1).
+    rewrite (preserve_inv_trans_wellformed _ σ1).
+    rewrite (preserve_inv_pgt_mb_consistent _ σ1).
     rewrite p_upd_pc_mem p_upd_reg_mem.
     all: try rewrite p_upd_pc_pgt p_upd_reg_pgt //.
     all: try rewrite p_upd_pc_trans p_upd_reg_trans //.
@@ -173,7 +174,8 @@ Proof.
     rewrite (preserve_get_retri_gmap _ σ1).
     rewrite (preserve_inv_trans_hpool_consistent _ σ1).
     rewrite (preserve_inv_trans_pgt_consistent _ σ1).
-    rewrite (preserve_inv_trans_pg_num_ub _ σ1).
+    rewrite (preserve_inv_trans_wellformed _ σ1).
+    rewrite (preserve_inv_pgt_mb_consistent _ σ1).
     rewrite p_upd_pc_mem p_upd_reg_mem.
     all: try rewrite p_upd_pc_pgt p_upd_reg_pgt //.
     all: try rewrite p_upd_pc_trans p_upd_reg_trans //.
